TypeSystemsInLean/PLFABasedSTLC/Preservation.lean
@@ -60,10 +60,7 @@ theorem preservation
 
   induction hs generalizing Γ A with
 
-  ----------------------------------------------------------------
   -- β
-  ----------------------------------------------------------------
-
   | beta hv =>
       cases ht with
       | ap hLam hArg =>
@@ -78,16 +75,12 @@ theorem preservation
                     intro x T h
                     cases h with
                     | here =>
-                        simpa [single]
-                          using hArg
+                        simpa [single] using hArg
                     | there h =>
                         exact HasType.var h)
                   hBody
 
-  ----------------------------------------------------------------
   -- app₁
-  ----------------------------------------------------------------
-
   | app₁ hs ih =>
       cases ht with
       | ap h₁ h₂ =>
@@ -95,15 +88,58 @@ theorem preservation
             (ih h₁)
             h₂
 
-  ----------------------------------------------------------------
   -- app₂
-  ----------------------------------------------------------------
-
   | app₂ hv hs ih =>
       cases ht with
       | ap h₁ h₂ =>
           exact HasType.ap
             h₁
             (ih h₂)
+
+  -- pair₁
+  | pair₁ hs ih =>
+      cases ht with
+      | pair h₁ h₂ =>
+          exact HasType.pair
+            (ih h₁)
+            h₂
+
+  -- pair₂
+  | pair₂ hv hs ih =>
+      cases ht with
+      | pair h₁ h₂ =>
+          exact HasType.pair
+            h₁
+            (ih h₂)
+
+  -- proj1₁
+  | proj1₁ hs ih =>
+      cases ht with
+      | proj1Ty h =>
+          exact HasType.proj1Ty
+            (ih h)
+
+  -- proj1Pair
+  | proj1Pair hv₁ hv₂ =>
+      cases ht with
+      | proj1Ty h =>
+          cases h with
+          | pair h₁ h₂ =>
+              exact h₁
+
+  -- proj2₁
+  | proj2₁ hs ih =>
+      cases ht with
+      | proj2Ty h =>
+          exact HasType.proj2Ty
+            (ih h)
+
+  -- proj2Pair
+  | proj2Pair hv₁ hv₂ =>
+      cases ht with
+      | proj2Ty h =>
+          cases h with
+          | pair h₁ h₂ =>
+              exact h₂
 
 end STLC
